TODO.md
@@ -1,3 +1,9 @@
 # TODO
-1. Implement runTc
-2. Implement typecheck
+1. Implement typecheck
+2. Write tests for typecheck & fix bugs from typecheck
+3. Write down what the type theory
+4. Consider the pros and cons of implementing beta reduction and beta equality
+5. Implement elaboration monad
+  a. Develop list of elaboration monad tactics
+  b. Implement skeleton of the elaboration monad
+  c. Implement elaboration monad tactics (add each tactic below)
